Moving over to proper_eutt_contains_ub.

src/coq/Theory/ContainsUB.v
@@ -1,5 +1,5 @@
 Require Import String.
-
+Definition blah := 2.
 From ITree Require Import
      ITree
      Basics
@@ -28,66 +28,13 @@ From Coq Require Import Relations RelationClasses.
 Require Import Morphisms.
 Require Import Paco.paco.
 
-Section contains_UB.
-  Context {E F G : Type -> Type}.
-  Local Notation Eff := (E +' F +' UBE +' G).
-
-  Inductive contains_UB' {R} (CUB : itree Eff R -> Prop) : itree' Eff R -> Prop :=
-  | CrawlTau  : forall t, CUB t -> contains_UB' CUB (TauF t)
-  | CrawlVis1 : forall Y (e : (E +' F) Y) x (k : Y -> itree Eff R), CUB (k x) -> contains_UB' CUB (VisF (subevent _ e) k)
-  | CrawlVis2 : forall Y (e : G Y) x (k : Y -> itree Eff R), CUB (k x) -> contains_UB' CUB (VisF (subevent _ e) k)
-  | FindUB    : forall s k, contains_UB' CUB (VisF (subevent _ (ThrowUB s)) k).
-
-  Definition contains_UB {R} : itree Eff R -> Prop
-    := paco1 (fun CUB t => contains_UB' CUB (observe t)) bot1.
-
-  Lemma contains_UB_mon {R} : monotone1 (fun (CUB : rel1 (itree Eff R)) (t : itree Eff R) => contains_UB' CUB (observe t)).
-  Proof.
-    unfold monotone1.
-    intros x0 r r' IN LE.
-    induction (observe x0).
-    - inversion IN.
-    - inversion IN; subst; constructor; eauto.
-    - inversion IN;
-        try apply inj_pair2 in H1;
-        try apply inj_pair2 in H2;
-        subst;
-        try econstructor; eauto.
-
-      apply inj_pair2 in H1.
-      apply inj_pair2 in H2.
-      subst.
-
-      econstructor.
-  Qed.
-End contains_UB.
-
-Hint Unfold contains_UB : Core.
-Hint Resolve contains_UB_mon : paco.
+Require Import Coq.Program.Equality.
 
 Ltac inv_existT :=
   repeat match goal with
          | H: existT _ _ _ = existT _ _ _ |- _ =>
              apply inj_pair2 in H; inversion H; subst
          end.
-
-Ltac inv_contains_UB :=
-  match goal with
-  | UB : contains_UB ?x,
-      H : _ = observe ?x |- _ =>
-      punfold UB; rewrite <- H in UB;
-      inversion UB; subst
-  | UB : contains_UB ?x
-    |- _ =>
-      punfold UB;
-      inversion UB; subst
-  end.
-
-Ltac pfold_contains_UB :=
-  match goal with
-  | H : _ = observe ?y |- paco1 _ _ ?y =>
-      pfold; rewrite <- H
-  end.
 
 Ltac inv_observes :=
   repeat
@@ -97,230 +44,339 @@ Ltac inv_observes :=
         setoid_rewrite <- H1 in H2; inversion H2; subst
     end.
 
-Ltac subst_into_contains_UB :=
-  match goal with
-  | OBS : _ = observe ?x,
-      CUB : contains_UB ?x |- _ =>
-      punfold CUB; subst_into_contains_UB
-  | OBS : _ = observe ?x,
-      CUB : contains_UB' _ (observe ?x) |- _ =>
-      setoid_rewrite <- OBS in CUB
-  end.
+Section contains_UB.
+  Context {E F G : Type -> Type}.
+  #[local] Notation Eff := (E +' F +' UBE +' G).
 
-Ltac inv_contains_UB' :=
-  match goal with
-  | CUB : contains_UB' _ _ |- _ =>
-      inversion CUB; subst
-  end.
+  Inductive contains_UB {R} : itree Eff R -> Prop :=
+  | CrawlTau  : forall t1 t2, t2 ≅ Tau t1 -> contains_UB t1 -> contains_UB t2
+  | CrawlVis1 : forall Y (e : (E +' F) Y) x k t2, t2 ≅ (vis e k) -> contains_UB (k x) -> contains_UB t2
+  | CrawlVis2 : forall Y (e : G Y) x k t2, t2 ≅ (vis e k) -> contains_UB (k x) -> contains_UB t2
+  | FindUB    : forall s k t2, t2 ≅ (vis (subevent _ (ThrowUB s)) k) -> contains_UB t2.
 
+  #[global] Instance proper_eutt_contains_UB {R} {RR : relation R} : Proper (@eqit Eff _ _ RR true true ==> iff) contains_UB.
+  Proof.
+    unfold Proper, respectful.
+    intros x y EQ.
+    split; intros UB.
+    { revert y EQ.
+      induction UB.
+      - intros y EQ.
+        apply IHUB.
+        rewrite <- (tau_eutt t1).
+        rewrite <- H.
+        auto.
+      - rename Y into T.
+        intros y EQ.
+        punfold EQ; red in EQ.
+        { remember (observe t2) as t2o.
+          remember (observe y) as yo.
+          revert e k t2 y H UB IHUB Heqt2o Heqyo.
+          induction EQ; intros e' k t2' y H UB IHUB Heqt2o Heqyo.
+          punfold H; red in H.
+          rewrite <- Heqt2o in H.
+          inversion H.
+
+          punfold H; red in H.
+          rewrite <- Heqt2o in H.
+          cbn in H.
+          inversion H; inversion CHECK.
+
+          - punfold H; red in H.
+            rewrite <- Heqt2o in H.
+            cbn in H.
+            dependent induction H.
+
+            eapply CrawlVis1 with (k0:=k2) (e:=subevent T e').
+            { symmetry.
+              pfold; red.
+              rewrite <- Heqyo.
+              constructor; eauto.
+              intros v.
+              red. left.
+              apply Reflexive_eqit. typeclasses eauto.
+            }
+
+            apply IHUB.
+            pclearbot.
+            rewrite <- REL0.
+            eauto.
+          - punfold H; red in H.
+            rewrite <- Heqt2o in H.
+            cbn in H.
+            inversion H; inversion CHECK0.
+          - punfold H; red in H.
+            cbn in H.
+            dependent induction H.
+            eapply CrawlTau with (t1 := t2).
+
+            pfold; red; rewrite <- Heqyo.
+            cbn.
+            constructor; left.
+            apply Reflexive_eqit. typeclasses eauto.
+            eapply IHEQ; eauto.
+            pfold; red; rewrite <- x.
+            cbn; constructor; eauto.
+        }
+      - rename Y into T.
+        intros y EQ.
+        punfold EQ; red in EQ.
+        { remember (observe t2) as t2o.
+          remember (observe y) as yo.
+          revert e k t2 y H UB IHUB Heqt2o Heqyo.
+          induction EQ; intros e' k t2' y H UB IHUB Heqt2o Heqyo.
+
+          punfold H; red in H.
+          rewrite <- Heqt2o in H.
+          inversion H.
+
+          punfold H; red in H.
+          rewrite <- Heqt2o in H.
+          cbn in H.
+          inversion H; inversion CHECK.
+
+          - punfold H; red in H.
+            rewrite <- Heqt2o in H.
+            cbn in H.
+            dependent induction H.
+
+            eapply CrawlVis2 with (k0:=k2).
+            { symmetry.
+              pfold; red.
+              rewrite <- Heqyo.
+              cbn.
+              econstructor; eauto.
+              intros v.
+              red. left.
+              apply Reflexive_eqit. typeclasses eauto.
+            }
+
+            apply IHUB.
+            pclearbot.
+            rewrite <- REL0.
+            eauto.
+          - punfold H; red in H.
+            rewrite <- Heqt2o in H.
+            cbn in H.
+            inversion H; inversion CHECK0.
+          - punfold H; red in H.
+            cbn in H.
+            dependent induction H.
+            eapply CrawlTau with (t1 := t2).
+
+            pfold; red; rewrite <- Heqyo.
+            cbn.
+            constructor; left.
+            apply Reflexive_eqit. typeclasses eauto.
+            eapply IHEQ; eauto.
+            pfold; red; rewrite <- x.
+            cbn; constructor; eauto.
+        }
+      - intros y EQ.
+        punfold H; red in H.
+        dependent induction H.
+        punfold EQ; red in EQ.
+        rewrite <- x in EQ.
+        dependent induction EQ.
+        + eapply FindUB.
+          pfold; red.
+          rewrite <- x.
+          cbn.
+          econstructor; intros [].
+        + eapply CrawlTau with (t1:=t0).
+          pfold; red; rewrite <- x; cbn.
+          constructor. left.
+          apply Reflexive_eqit. typeclasses eauto.
+
+          eapply IHEQ; eauto.          
+    }
+
+    { revert x EQ.
+      induction UB.
+      - intros x EQ.
+        apply IHUB.
+        rewrite <- (tau_eutt t1).
+        rewrite <- H.
+        auto.
+      - rename Y into T.
+        rename x into v.
+        intros x EQ.
+        punfold EQ; red in EQ.
+        { remember (observe t2) as t2o.
+          remember (observe x) as xo.
+          revert e k t2 x H UB IHUB Heqt2o Heqxo.
+          induction EQ; intros e' k t2' x H UB IHUB Heqt2o Heqxo.
+          punfold H; red in H.
+          rewrite <- Heqt2o in H.
+          inversion H.
+
+          punfold H; red in H.
+          rewrite <- Heqt2o in H.
+          cbn in H.
+          inversion H; inversion CHECK.
+
+          - punfold H; red in H.
+            rewrite <- Heqt2o in H.
+            cbn in H.
+            dependent induction H.
+
+            eapply CrawlVis1 with (k0:=k1) (e:=subevent T e').
+            { symmetry.
+              pfold; red.
+              rewrite <- Heqxo.
+              constructor; eauto.
+              intros v'.
+              red. left.
+              apply Reflexive_eqit. typeclasses eauto.
+            }
+
+            apply IHUB.
+            pclearbot.
+            rewrite <- REL0.
+            eauto.
+          - punfold H; red in H.
+            cbn in H.
+            dependent induction H.
+            eapply CrawlTau with (t2 := t1).
+
+            pfold; red; rewrite <- Heqxo.
+            cbn.
+            constructor; left.
+            apply Reflexive_eqit. typeclasses eauto.
+            eapply IHEQ; eauto.
+            pfold; red; rewrite <- x.
+            cbn; constructor; eauto.
+          - punfold H; red in H.
+            rewrite <- Heqt2o in H.
+            cbn in H.
+            inversion H; inversion CHECK0.
+        }
+      - rename Y into T.
+        intros y EQ.
+        punfold EQ; red in EQ.
+        { remember (observe t2) as t2o.
+          remember (observe y) as yo.
+          revert e k t2 y H UB IHUB Heqt2o Heqyo.
+          induction EQ; intros e' k t2' y H UB IHUB Heqt2o Heqyo.
+
+          punfold H; red in H.
+          rewrite <- Heqt2o in H.
+          inversion H.
+
+          punfold H; red in H.
+          rewrite <- Heqt2o in H.
+          cbn in H.
+          inversion H; inversion CHECK.
+
+          - punfold H; red in H.
+            rewrite <- Heqt2o in H.
+            cbn in H.
+            dependent induction H.
+
+            eapply CrawlVis2 with (k0:=k1).
+            { symmetry.
+              pfold; red.
+              rewrite <- Heqyo.
+              cbn.
+              econstructor; eauto.
+              intros v.
+              red. left.
+              apply Reflexive_eqit. typeclasses eauto.
+            }
+
+            apply IHUB.
+            pclearbot.
+            rewrite <- REL0.
+            eauto.
+          - punfold H; red in H.
+            cbn in H.
+            dependent induction H.
+            eapply CrawlTau with (t2 := t1).
+
+            pfold; red; rewrite <- Heqyo.
+            cbn.
+            constructor; left.
+            apply Reflexive_eqit. typeclasses eauto.
+            eapply IHEQ; eauto.
+            pfold; red; rewrite <- x.
+            cbn; constructor; eauto.
+          - punfold H; red in H.
+            rewrite <- Heqt2o in H.
+            cbn in H.
+            inversion H; inversion CHECK0.
+        }
+      - intros y EQ.
+        punfold H; red in H.
+        dependent induction H.
+        punfold EQ; red in EQ.
+        rewrite <- x in EQ.
+        dependent induction EQ.
+        + eapply FindUB.
+          pfold; red.
+          rewrite <- x.
+          cbn.
+          econstructor; intros [].
+        + eapply CrawlTau with (t3:=t1).
+          pfold; red; rewrite <- x; cbn.
+          constructor. left.
+          apply Reflexive_eqit. typeclasses eauto.
+
+          eapply IHEQ; eauto.          
+    }
+
+    Unshelve.
+
+    all: intros [].
+  Qed.
+
+  (*
+  (* TODO: Move this *)
+  Definition stronger (x1 x2 b : bool) : Prop :=
+    match b with
+    | true =>
+        (* Can remove taus, so anything is stronger *)
+        True
+    | false =>
+        (* Can't remove taus *)
+        match x1, x2 with
+        | false, false =>
+            True
+        | _, _ =>
+            False
+        end
+    end.
+
+  #[global] Instance eqit_eqit_Proper :
+    forall {E : Type -> Type} {R : Type} {RR : R -> R -> Prop} (bx1 bx2 by1 by2 b1 b2 : bool),
+      stronger bx1 bx2 b1 ->
+      stronger by1 by2 b2 ->
+      Proper (eqit RR bx1 bx2 ==> eqit RR by1 by2 ==> iff) (@eqit E _ _ RR b1 b2).
+  Proof.
+    intros E0 R RR bx1 bx2 by1 by2 b1 b2 STRONGX STRONGY.
+    unfold Proper, respectful.
+    intros x x' XX y y' YY.
+    split; intros XY.
+    { destruct bx1, bx2, b1; inversion STRONGX.
+      - rewrite XX in XY.
+
+    }
+    
+  Qed.
+*)
+
+End contains_UB.
 
 Section contains_UB_lemmas.
   Context {E F G : Type -> Type}.
   Local Notation Eff := (E +' F +' UBE +' G).
 
-  Lemma contains_UB_tau {R} (t : itree Eff R):
-    contains_UB t <-> contains_UB (Tau t).
-  Proof.
-    split; intros UB.
-    { pfold.
-      punfold UB.
-      constructor.
-      left.
-      pfold.
-      apply UB.
-    }
-
-    { pfold.
-      pinversion UB; subst.
-      punfold H0.
-    }
-  Qed.
-
   Lemma ret_not_contains_UB {R} {RR : relation R} :
-    forall (t : itree Eff R) rv a b, eqit RR a b t (ret rv) -> ~ contains_UB t.
+    forall (t : itree Eff R) rv, eqit RR true true t (ret rv) -> ~ contains_UB t.
   Proof.
-    intros t rv a b EQ CUB.
-    punfold EQ.
-    unfold eqit_ in EQ.
-    punfold CUB.
-    remember (observe t) as to.
-    remember (observe (ret rv)) as ro.
-    revert t Heqto Heqro.
-    induction EQ; intros t TO RO; inversion TO; inversion RO; subst.
-    - inversion CUB.
-    - eapply IHEQ.
-      + inversion CUB; subst; pclearbot.
-        punfold H2.
-      + reflexivity.
-      + reflexivity.
-  Qed.
-
-  Instance proper_eqit_contains_UB {R} {RR : relation R} (a b : bool) : Proper (@eqit Eff _ _ RR a b ==> iff) contains_UB.
-  Proof.
-    unfold Proper, respectful.
-    intros x y EQ.
-    split.
-    { generalize dependent RR.
-      generalize dependent y.
-      generalize dependent x.
-      pcofix CIH.
-      intros x y RR EQ UB.
-
-      pinversion EQ; subst;
-        inv_contains_UB;
-        inv_existT;
-        pclearbot;
-        try solve [
-            pfold_contains_UB;
-            econstructor; right; eauto
-          ]; inversion CHECK; subst.
-
-      - (* Left tau, nothing about y *)
-        clear UB.
-        punfold H1.
-
-        genobs y yo.
-        genobs t1 t1o.
-
-        (* revert H0. *)
-        clear H0.
-        revert t1 Heqt1o Heqyo.
-        pfold.
-
-        induction REL; intros t1' Heqt1o Heqyo; pose proof True as H0; inversion Heqt1o; inversion Heqyo; subst.
-        + inversion H1.
-        + inversion H1; subst; pclearbot.
-          constructor.
-          right.
-          rewrite H2 in H1.
-          eapply CIH.
-          2: pfold; apply H1.
-
-          punfold REL.
-          red in REL.
-          pfold.
-          red.
-          rewrite <- H2.
-          constructor.
-          constructor.
-          eauto.
-        + inversion H1; subst; inv_existT; subst; pclearbot;
-            econstructor; right; eauto.
-        + inversion H1; subst; pclearbot.
-          punfold H4.
-        + constructor.
-          right.
-          eapply CIH; eauto.
-          pfold.
-          auto.
-      - (* Left and right tau *)
-        pfold_contains_UB.
-        constructor; right; eapply CIH;
-          pfold; eauto.
-      - (* Right tau, external call on the left *)
-        pfold_contains_UB.
-        constructor; right; eapply CIH;
-          pfold; eauto.
-      - (* Right tau, debug or failure event on the left *)
-        pfold_contains_UB.
-        constructor; right; eapply CIH;
-          pfold; eauto.
-      - (* UB *)
-        pfold.
-        rewrite <- H1.
-        constructor.
-        right.
-        eapply CIH.
-        pfold.
-        red.
-        apply REL.
-        pfold.
-        auto.
-    }
-
-    { generalize dependent RR.
-      generalize dependent x.
-      generalize dependent y.
-      pcofix CIH.
-      intros y x RR EQ UB.
-
-      pinversion EQ; subst;
-        inv_contains_UB;
-        inv_existT;
-        pclearbot;
-        try solve [
-            pfold_contains_UB;
-            econstructor; right; eauto
-          ]; inversion CHECK; subst.
-
-      - (* Left and right tau *)
-        pfold_contains_UB.
-        constructor; right; eapply CIH;
-          pfold; eauto.
-      - (* Left tau, external call on the right *)
-        pfold_contains_UB.
-        constructor; right; eapply CIH;
-          pfold; eauto.
-      - (* Left tau, debug or failure on the right *)
-        pfold_contains_UB.
-        constructor; right; eapply CIH;
-          pfold; eauto.
-      - (* UB *)
-        pfold_contains_UB.
-        constructor; right; eapply CIH;
-          pfold; eauto.
-      - (* Left tau, nothing about x on the right. *)
-        clear UB.
-        punfold H0.
-
-        genobs x xo.
-        genobs t2 t2o.
-
-        (* revert H0. *)
-        clear H1.
-        revert t2 Heqt2o Heqxo.
-        pfold.
-
-        induction REL; intros t2' Heqt2o Heqxo; pose proof True as H1; inversion Heqt2o; inversion Heqxo; subst.
-        + inversion H0.
-        + inversion H0; subst; pclearbot.
-          constructor.
-          right.
-          rewrite H2 in H0.
-          eapply CIH.
-          2: pfold; apply H0.
-
-          punfold REL.
-          red in REL.
-          pfold.
-          red.
-          rewrite <- H2.
-          constructor.
-          constructor.
-          eauto.
-        + inversion H0; subst; inv_existT; subst; pclearbot;
-            econstructor; right; eauto.
-        + constructor.
-          right.
-          eapply CIH; eauto.
-          pfold.
-          auto.
-        + inversion H0; subst; pclearbot.
-          punfold H4.
-    }
-  Qed.
-
-  Hint Resolve interp_PropT__mono : paco.
-
-  Lemma contains_UB_eutt :
-    forall R (RR : relation R) (t1 t2 : itree Eff R),
-      contains_UB t1 ->
-      eutt RR t2 t1 ->
-      contains_UB t2.
-  Proof.
-    intros R RR t1 t2 UB EQ.
-    rewrite EQ.
-    eauto.
+    intros t rv EQ CUB.
+    rewrite EQ in CUB.
+    inversion CUB; subst;
+      pinversion H; inversion CHECK.
   Qed.
 
 End contains_UB_lemmas.
@@ -330,7 +386,7 @@ Section refine_OOM_h_lemmas.
   Local Notation Eff := (E +' OOME +' UBE +' G).
 
   (* Only the <- direction is true *)
-  Instance proper_refine_OOM_h
+  Global Instance proper_refine_OOM_h
            {R} {RR : relation R} : Proper (@refine_OOM_h E (UBE +' G) _ RR ==> flip impl) contains_UB.
   Proof.
     unfold Proper, respectful.
@@ -369,3 +425,74 @@ Lemma eqitree_inv_Tau_l {E R} (t t' : itree E R) :
 Proof.
   intros; punfold H; inv H; try inv CHECK; pclearbot; eauto.
 Qed.
+
+Section bind_lemmas.
+  Context {E F G : Type -> Type}.
+  Local Notation Eff := (E +' F +' UBE +' G).
+
+  Lemma bind_contains_UB :
+    forall {R T} (t : itree Eff R) (k : R -> itree Eff T),
+      contains_UB t ->
+      contains_UB (ITree.bind t k).
+  Proof.
+    intros R T t k CUB.
+  Admitted.
+
+  Lemma bind_contains_UB' :
+    forall {R T} (t : itree Eff R) (k : R -> itree Eff T),
+      contains_UB (ITree.bind t k) ->
+      (forall x, ~ contains_UB (k x)) ->
+      contains_UB t.
+  Proof.
+
+  Admitted.
+End bind_lemmas.
+
+Section interp_lemmas.
+  Context {E1 F1 G1 : Type -> Type}.
+  Local Notation Eff1 := (E1 +' F1 +' UBE +' G1).
+
+  Context {E2 F2 G2 : Type -> Type}.
+  Local Notation Eff2 := (E2 +' F2 +' UBE +' G2).
+
+  Variable (handler : Handler Eff1 Eff2).
+
+  Definition handler_keeps_UB :=
+    forall {R} (e : UBE R),
+      contains_UB (handler _ ((inr1 (inr1 (inl1 e))) : Eff1 R)).
+
+  Lemma interp_contains_UB :
+    forall {R} (t : itree Eff1 R),
+      contains_UB t ->
+      handler_keeps_UB ->
+      contains_UB (interp handler t).
+  Proof.
+    intros R t UB KEEP.
+
+    unfold handler_keeps_UB in KEEP.
+
+    rewrite (itree_eta t).
+    genobs t to.
+    revert t to Heqto UB.
+    pcofix CIH; intros t to Heqto UB.
+
+    pinversion UB; clear UB.
+    - (* Tau *)
+      admit.
+    - (* Vis E + F *)
+      admit.
+    - (* Vis G *)
+      admit.
+    - (* UB *)
+      rewrite <- H0 in Heqto.
+      subst.
+      pfold.
+
+      unfold handler_keeps_UB in KEEP.
+      pose proof (KEEP _ (ThrowUB s)).
+      rewrite <- InterpFacts.interp_trigger in H.
+
+      punfold H.
+      cbn in H.
+  Admitted.
+End interp_lemmas.
